Split into multiple theories

Skel.thy
@@ -1,92 +1,53 @@
 theory Skel
-imports Main
+imports Main Scalar Exp
 begin
 
-type_synonym 'a array = "'a list"
+datatype result = Res const | Error
 
-datatype scalar_unary = Inc | Dec
+type_synonym env = "(var \<times> const) list"
 
-datatype scalar_binary = Add | Mul | Sub
+fun res_cons :: "result \<Rightarrow> result \<Rightarrow> result" where
+  "res_cons (Res a1) (Res (ArrayC a2)) = Res (ArrayC (a1 # a2))" |
+  "res_cons _ _ = Error"
 
-datatype scalar_const = IntC int
+fun apply_map :: "('a \<Rightarrow> result) \<Rightarrow> 'a array \<Rightarrow> result" where
+  "apply_map f [] = Res (ArrayC [])" |
+  "apply_map f (x # xs) = res_cons (f x) (apply_map f xs)"
 
-fun eval_scalar_unary :: "scalar_unary \<Rightarrow> scalar_const \<Rightarrow> scalar_const" where
-  "eval_scalar_unary Inc (IntC n) = IntC (n + 1)" |
-  "eval_scalar_unary Dec (IntC n) = IntC (n - 1)"
-
-fun eval_scalar_binary :: "scalar_binary \<Rightarrow> scalar_const \<Rightarrow> scalar_const \<Rightarrow> scalar_const" where
-  "eval_scalar_binary Add (IntC i) (IntC j) = IntC (i + j)" |
-  "eval_scalar_binary Mul (IntC i) (IntC j) = IntC (i * j)" |
-  "eval_scalar_binary Sub (IntC i) (IntC j) = IntC (i - j)"
-
-type_synonym var = string
-
-datatype exp = Const scalar_const
-  | Unary scalar_unary exp
-  | Binary scalar_binary exp exp
-  | Var var
-  | Array "exp array"
-  | Map var exp exp 
-  | Zip exp exp 
-  | Reduce var var exp exp exp
-  | Split exp exp 
-  | Join exp
-
-datatype result = Res exp | Error
-
-type_synonym env = "(var \<times> exp) list"
+fun apply_zip :: "const array \<Rightarrow> const array \<Rightarrow> result" 
+and make_tuple :: "(const \<times> const) \<Rightarrow> const" where
+  "apply_zip xs ys = Res (ArrayC (map make_tuple (zip xs ys)))" |
+  "make_tuple (c1, c2) = TupleC c1 c2"
 
 fun lookup :: "'a \<Rightarrow> ('a \<times> 'b) list \<Rightarrow> 'b option" where
   "lookup k [] = None" |
   "lookup k ((k',v)#ls) = (if k = k' then Some v else lookup k ls)"
 
-primrec error_to_zero :: "result \<Rightarrow> exp" where
-  "error_to_zero (Res e) = e" |
-  "error_to_zero Error = Const (IntC 0)"
-
-primrec any_errors :: "result list \<Rightarrow> bool" where
-  "any_errors [] = False" |
-  "any_errors (x # xs) =
-    (case x of 
-      Res _ \<Rightarrow> any_errors xs
-    | Error \<Rightarrow> True)"
-
 fun interp :: "exp \<Rightarrow> env \<Rightarrow> result" where
-  "interp (Const c) \<rho> = Res (Const c)" |
+  "interp (Const c) \<rho> = Res c" |
   "interp (Unary p e) \<rho> = (case interp e \<rho> of 
-                            Res (Const c) \<Rightarrow> Res (Const (eval_scalar_unary p c))
+                            Res (ScalarC c) \<Rightarrow> Res (ScalarC (eval_scalar_unary p c))
                           | Error \<Rightarrow> Error)" |
   "interp (Binary p e1 e2) \<rho> = (case (interp e1 \<rho>, interp e2 \<rho>) of
-                                 (Res (Const c1), Res (Const c2)) \<Rightarrow> 
-                                    Res (Const (eval_scalar_binary p c1 c2))
+                                 (Res (ScalarC c1), Res (ScalarC c2)) \<Rightarrow> 
+                                    Res (ScalarC (eval_scalar_binary p c1 c2))
                                | (Error,_) \<Rightarrow> Error | (_,Error) \<Rightarrow> Error)" |
   "interp (Var x) \<rho> = (case (lookup x \<rho>) of 
                         Some e \<Rightarrow> Res e
                       | None \<Rightarrow> Error)" |
-  "interp (Array ve) \<rho> = Res (Array (map (\<lambda>i. error_to_zero (interp i \<rho>)) ve))" |
+  "interp (Array []) _ = Res (ArrayC [])" |
+  "interp (Array (x # xs)) \<rho> = res_cons (interp x \<rho>) (interp (Array xs) \<rho>)" |
   "interp (Map v le ve) \<rho> = 
     (case (interp ve \<rho>) of 
-      Res (Array a) \<Rightarrow> let a' = (map (\<lambda>i. interp le ((v,i)#\<rho>)) a)
-                       in if (any_errors a') 
-                          then Error 
-                          else Res (Array (map (\<lambda>i. error_to_zero i) a'))
+      Res (ArrayC a) \<Rightarrow> apply_map (\<lambda>i. interp le ((v,i)#\<rho>)) a
     | Error \<Rightarrow> Error)" |
+  "interp (Zip e1 e2) \<rho> =
+    (case (interp e1 \<rho>, interp e2 \<rho>) of 
+      (Res (ArrayC a1), Res (ArrayC a2)) \<Rightarrow> apply_zip a1 a2
+    | (Error,_) \<Rightarrow> Error | (_,Error) \<Rightarrow> Error)" |
   "interp _ \<rho> = Error"
 
 definition eval :: "exp \<Rightarrow> result" where "eval e = interp e []"
 declare eval_def[simp]
 
-(* sanity checking the interpreter *)
-
-abbreviation p0 :: exp where "p0 \<equiv> Binary Add (Const (IntC 1)) (Const (IntC 2))"
-abbreviation p1 :: exp where "p1 \<equiv> Unary Inc (Const (IntC 2))"
-abbreviation p2 :: exp where "p2 \<equiv> Array [p0, p1]"
-theorem "eval (Map x (Unary Inc (Var x)) p2) = 
-         Res (Array [Const (IntC 4), Const (IntC 4)])"
-by fastforce
-theorem "eval (Map x (Binary Add (Var x) (Const (IntC 1))) p2) = 
-         Res (Array [Const (IntC 4), Const (IntC 4)])"
-by fastforce
-theorem "eval (Map x (Binary Mul (Var x) (Var x)) p2) = 
-         Res (Array [Const (IntC 9), Const (IntC 9)])"
-by fastforce
+end
