Exp.thy
@@ -1,0 +1,25 @@
+theory Exp
+imports Main Scalar
+begin
+
+type_synonym 'a array = "'a list"
+
+datatype const = ScalarC scalar_const | TupleC const const | ArrayC "const array"
+
+type_synonym var = string
+
+datatype exp = Const const
+  | Unary scalar_unary exp
+  | Binary scalar_binary exp exp
+  | PrjL exp
+  | PrjR exp
+  | Tuple exp exp
+  | Array "exp array"
+  | Var var
+  | Map var exp exp 
+  | Zip exp exp 
+  | Reduce var var exp exp exp
+  | Split exp exp 
+  | Join exp
+
+end
