Test.thy
@@ -1,0 +1,21 @@
+theory Test
+imports Main Skel
+begin
+
+(* sanity checking the interpreter *)
+abbreviation p0 :: exp where "p0 \<equiv> Binary Add (Const (ScalarC (IntC 1))) (Const (ScalarC (IntC 2)))"
+abbreviation p1 :: exp where "p1 \<equiv> Unary Inc (Const (ScalarC (IntC 2)))"
+abbreviation p2 :: exp where "p2 \<equiv> Array [p0, p1]"
+theorem "eval (Map x (Unary Inc (Var x)) p2) = 
+         Res (ArrayC [(ScalarC (IntC 4)), (ScalarC (IntC 4))])"
+by fastforce
+theorem "eval (Map x (Binary Add (Var x) (Const (ScalarC (IntC 1)))) p2) = 
+         Res (ArrayC [(ScalarC (IntC 4)), (ScalarC (IntC 4))])"
+by fastforce
+theorem "eval (Map x (Binary Mul (Var x) (Var x)) p2) = 
+         Res (ArrayC [ScalarC (IntC 9), ScalarC (IntC 9)])"
+by fastforce
+theorem "eval (Zip p2 p2) = 
+         Res (ArrayC [TupleC (ScalarC (IntC 3)) (ScalarC (IntC 3)), 
+                      TupleC (ScalarC (IntC 3)) (ScalarC (IntC 3))])"
+by fastforce
